Refinements of weak approximations
Signed-off-by: zeramorphic <zeramorphic@proton.me>

src/phase2/litter_completion.lean
@@ -1,6 +1,6 @@
+import phase2.flexible_completion
 import phase2.reduction
-import phase2.supported_action
-import phase2.weak_approx
+import phase2.refine
 
 open quiver set sum with_bot
 open_locale classical
@@ -16,19 +16,10 @@ variables [params.{u}] {α : Λ} [position_data.{}] [phase_2_assumptions α] {β
   (H : hypothesis ⟨inr (f_map (coe_ne_coe.mpr $ coe_ne' hδε) t).to_near_litter,
     (A.cons (coe_lt hε)).cons (bot_lt_coe _)⟩)
 
-def lawful_atom_map (π₀ : struct_approx β) (π : allowable β) : Prop :=
-∀ (a : atom) (A : extended_index β) (h : a ∉ (π₀ A).atom_perm.domain),
-  struct_perm.derivative A π.to_struct_perm • a =
-  ((π₀ A).largest_sublitter a.1).order_iso
-  ((π₀ A).largest_sublitter (struct_perm.derivative A π.to_struct_perm • a.1))
-  ⟨a, (π₀ A).mem_largest_sublitter_of_not_mem_domain a h⟩
-
 /-- The inductive hypothesis used for proving freedom of action:
-Every free approximation exactly approximates some allowable permutation, and its action on atoms
-not in the domain of the approximation is given by the order isomorphism between sublitters. -/
+Every free approximation exactly approximates some allowable permutation. -/
 def foa_ih (β : Iic α) : Prop :=
-∀ (π₀ : struct_approx β), π₀.free →
-  ∃ (π : allowable β), π₀.exactly_approximates π.to_struct_perm ∧ π₀.lawful_atom_map π
+∀ (π₀ : struct_approx β), π₀.free → ∃ (π : allowable β), π₀.exactly_approximates π.to_struct_perm
 
 /-- A proof-relevant statement that `L` is `A`-inflexible (excluding `ε = ⊥`). -/
 structure inflexible_coe (L : litter) (A : extended_index β) :=
@@ -165,6 +156,13 @@ structure hypothesis_injective_inflexible {L : litter} {A : extended_index β}
     (by rwa [inflexible_support, ← h.hL, ← h.hA] at ha) =
   H.atom_image b ((h.B.cons (coe_lt h.hδ)).comp B)
     (by rwa [inflexible_support, ← h.hL, ← h.hA] at hb) → a = b)
+(litter_map_injective : ∀ (L₁ L₂ : litter) B
+  (hL₁ : (inr L₁.to_near_litter, B) ∈ inflexible_support h)
+  (hL₂ : (inr L₂.to_near_litter, B) ∈ inflexible_support h),
+  (H.near_litter_image L₁.to_near_litter ((h.B.cons (coe_lt h.hδ)).comp B)
+    (by rwa [inflexible_support, ← h.hL, ← h.hA] at hL₁) ∩
+  H.near_litter_image L₂.to_near_litter ((h.B.cons (coe_lt h.hδ)).comp B)
+    (by rwa [inflexible_support, ← h.hL, ← h.hA] at hL₂) : set atom).nonempty → L₁ = L₂)
 (atom_mem : ∀ a (L : litter) B
   (ha : (inl a, B) ∈ inflexible_support h) (hL : (inr L.to_near_litter, B) ∈ inflexible_support h),
   a ∈ litter_set L ↔
@@ -199,24 +197,27 @@ def hypothesised_weak_struct_approx {L : litter} {A : extended_index β}
     exact h,
   end,
   atom_map_injective := λ a b ha hb, hH.atom_map_injective a b B ha hb,
-  litter_map_injective := sorry,
+  litter_map_injective := λ L₁ L₂ hL₁ hL₂, hH.litter_map_injective L₁ L₂ B hL₁ hL₂,
   atom_mem := λ a ha L hL, hH.atom_mem a L B ha hL,
 }
 
 @[simp] lemma hypothesised_weak_struct_approx_atom_map {L : litter} {A : extended_index β}
   (H : hypothesis ⟨inr L.to_near_litter, A⟩) (h : inflexible_coe L A)
   (hH : hypothesis_injective_inflexible H h) (B : extended_index h.δ) (a : atom) :
-  (hypothesised_weak_struct_approx H h hH B).atom_map a = ⟨(inl a, B) ∈ inflexible_support h,
-    λ ha, H.atom_image a ((h.B.cons (coe_lt h.hδ)).comp B)
-      (by rwa [inflexible_support, ← h.hL, ← h.hA] at ha)⟩ := rfl
+  (hypothesised_weak_struct_approx H h hH B).atom_map a = {
+    dom := (inl a, B) ∈ inflexible_support h,
+    get := λ ha, H.atom_image a ((h.B.cons (coe_lt h.hδ)).comp B)
+      (by rwa [inflexible_support, ← h.hL, ← h.hA] at ha)
+  } := rfl
 
 @[simp] lemma hypothesised_weak_struct_approx_litter_map {L : litter} {A : extended_index β}
   (H : hypothesis ⟨inr L.to_near_litter, A⟩) (h : inflexible_coe L A)
   (hH : hypothesis_injective_inflexible H h) (B : extended_index h.δ) (L : litter) :
-  (hypothesised_weak_struct_approx H h hH B).litter_map L =
-  ⟨(inr L.to_near_litter, B) ∈ inflexible_support h,
-    λ hL, H.near_litter_image L.to_near_litter ((h.B.cons (coe_lt h.hδ)).comp B)
-      (by rwa [inflexible_support, ← h.hL, ← h.hA] at hL)⟩ := rfl
+  (hypothesised_weak_struct_approx H h hH B).litter_map L = {
+    dom := (inr L.to_near_litter, B) ∈ inflexible_support h,
+    get := λ hL, H.near_litter_image L.to_near_litter ((h.B.cons (coe_lt h.hδ)).comp B)
+      (by rwa [inflexible_support, ← h.hL, ← h.hA] at hL)
+  } := rfl
 
 noncomputable def litter_perm_below (π : struct_approx β) {γ : Iic α} {δ : Iio α}
   (hδ : (δ : Λ) < γ) (B : path (β : type_index) γ) : extended_index δ → local_perm litter :=
@@ -227,7 +228,7 @@ lemma hypothesised_weak_struct_approx_free (π : struct_approx β) (hπ : π.fre
   {A : extended_index β} (H : hypothesis ⟨inr L.to_near_litter, A⟩) (h : inflexible_coe L A)
   (hH : hypothesis_injective_inflexible H h) :
   @struct_approx.free _ _ _ _ (h.δ : Iic α)
-  ((hypothesised_weak_struct_approx H h hH).complete (litter_perm_below π h.hδ h.B)) :=
+  ((hypothesised_weak_struct_approx H h hH).refine.complete (litter_perm_below π h.hδ h.B)) :=
 begin
   intros B L' hL',
   cases hL',
@@ -250,17 +251,7 @@ lemma allowable_of_weak_struct_approx_exactly_approximates (π : struct_approx �
   (w.complete (litter_perm_below π hδ B))
     .exactly_approximates (allowable_of_weak_struct_approx π hπ hδ B w hw).to_struct_perm :=
 (freedom_of_action_of_lt (δ : Iic α)
-  (hδ.trans_le (show _, from coe_le_coe.mp (le_of_path B))) _ hw).some_spec.1
-
--- lemma supported_perm_of_support_map_lawful_atom_map (π : struct_approx β) (hπ : π.free)
---   {γ : Iic α} {δ : Iio α} (hδ : (δ : Λ) < γ) (B : path (β : type_index) γ) (S : support_map δ)
---   (hS : (show struct_approx (δ : Iic α), from supported_action S
---     (λ (C : extended_index δ), π ((B.cons $ coe_lt hδ).comp C))).free) :
---   (show struct_approx (δ : Iic α), from supported_action S
---     (λ C, π ((B.cons $ coe_lt hδ).comp C))).lawful_atom_map
---   (supported_perm_of_support_map π hπ hδ B S hS) :=
--- (freedom_of_action_of_lt (δ : Iic α)
---   (hδ.trans_le (show _, from coe_le_coe.mp (le_of_path B))) _ hS).some_spec.2
+  (hδ.trans_le (show _, from coe_le_coe.mp (le_of_path B))) _ hw).some_spec
 
 noncomputable def hypothesised_allowable (π : struct_approx β) (hπ : π.free)
   {L : litter} {A : extended_index β} (h : inflexible_coe L A)
@@ -271,18 +262,10 @@ allowable_of_weak_struct_approx π hπ h.hδ h.B _ (hypothesised_weak_struct_app
 lemma hypothesised_allowable_exactly_approximates (π : struct_approx β) (hπ : π.free)
   {L : litter} {A : extended_index β} (h : inflexible_coe L A)
   (H : hypothesis ⟨inr L.to_near_litter, A⟩) (hH : hypothesis_injective_inflexible H h) :
-  ((hypothesised_weak_struct_approx H h hH).complete (litter_perm_below π h.hδ h.B))
+  ((hypothesised_weak_struct_approx H h hH).refine.complete (litter_perm_below π h.hδ h.B))
     .exactly_approximates (hypothesised_allowable π hπ h H hH).to_struct_perm :=
 allowable_of_weak_struct_approx_exactly_approximates π hπ h.hδ h.B _
   (hypothesised_weak_struct_approx_free π hπ H h hH)
-
--- lemma supported_perm_lawful_atom_map (π : struct_approx β) (hπ : π.free)
---   {L : litter} {A : extended_index β} (h : inflexible_coe L A)
---   (H : hypothesis ⟨inr L.to_near_litter, A⟩) :
---   (show struct_approx (h.δ : Iic α), from supported_action
---     (inflexible_support_map H h) (λ C, π ((h.B.cons $ coe_lt h.hδ).comp C))).lawful_atom_map
---   (supported_perm π hπ h H) :=
--- supported_perm_of_support_map_lawful_atom_map π hπ h.hδ h.B _ (π.litter_approx_free hπ H h)
 
 -- TODO: Rename next few lemmas.
 -- TODO: Trim assumptions from lots of these little lemmas, then package into `variables`.
@@ -295,415 +278,6 @@ lemma mem_inflexible_support (π : struct_approx β) (hπ : π.free)
 relation.trans_gen.tail'
   (refl_trans_gen_constrains_comp hd₂ _)
   (constrains.f_map h.hδ h.hε h.hδε h.B h.t d hd₁)
-
-/- lemma supported_perm_smul_atom_eq (π : struct_approx β) (hπ : π.free)
-  {L : litter} {A : extended_index β} (h : inflexible_coe L A)
-  (H : hypothesis ⟨inr L.to_near_litter, A⟩) (S : support_map h.δ)
-  (hS₁ : (show struct_approx (h.δ : Iic α), from
-    supported_action S (λ (B : extended_index h.δ), π ((h.B.cons $ coe_lt h.hδ).comp B))).free)
-  (hS₂ : inflexible_support_map H h ≤ S)
-  (hS₃ : ∀ B, S.injective B)
-  (d : support_condition h.δ) (hd₁ : d ∈ designated_support h.t)
-  (B : extended_index h.δ) (a : atom)
-  (hd₂ : relation.refl_trans_gen (constrains α h.δ) (inl a, B) d) :
-  struct_perm.derivative B (π.supported_perm_of_support_map hπ h.hδ h.B S hS₁).to_struct_perm • a =
-  struct_perm.derivative B (π.supported_perm hπ h H).to_struct_perm • a :=
-begin
-  have := mem_inflexible_support π hπ h B a d hd₁ hd₂,
-  rw [← struct_perm.of_bot_smul, ← struct_perm.of_bot_smul,
-    ← (supported_perm_exactly_approximates π hπ h H B).map_atom,
-    ← (supported_perm_of_support_map_exactly_approximates π hπ h.hδ h.B S hS₁ B).map_atom a _,
-    supported_action_smul_atom_eq, supported_action_smul_atom_eq],
-  refine (hS₂.map_atom _).symm,
-  { exact this, },
-  { exact (hS₃ B).le hS₂, },
-  { exact hS₃ B, },
-  { rw supported_action_atom_perm_domain_eq _ (hS₃ B),
-    exact or.inl (or.inl (or.inl (or.inl (hS₂.carrier_subset this)))), },
-  { rw supported_action_atom_perm_domain_eq _ ((hS₃ B).le hS₂),
-    exact or.inl (or.inl (or.inl (or.inl this))), },
-end
-
-lemma supported_perm_smul_litter_eq (π : struct_approx β) (hπ : π.free)
-  {L : litter} {A : extended_index β} (h : inflexible_coe L A)
-  (H : hypothesis ⟨inr L.to_near_litter, A⟩) (S : support_map h.δ)
-  (hS₁ : (show struct_approx (h.δ : Iic α), from
-    supported_action S (λ (B : extended_index h.δ), π ((h.B.cons $ coe_lt h.hδ).comp B))).free)
-  (hS₂ : inflexible_support_map H h ≤ S) (hS₃ : ∀ B, S.injective B)
-  (d : support_condition h.δ) (hd₁ : d ∈ designated_support h.t)
-  (B : extended_index h.δ) (L' : litter)
-  (ih : ∀ (y : support_condition h.δ), y ≺[α] (inr L'.to_near_litter, B) →
-    (∃ d ∈ designated_support h.t, relation.refl_trans_gen (constrains α h.δ) y d) →
-    π.supported_perm_of_support_map hπ h.hδ h.B S hS₁ • y =
-      π.supported_perm hπ h H • y)
-  (hd₂ : relation.refl_trans_gen (constrains α h.δ) (inr L'.to_near_litter, B) d) :
-  struct_perm.derivative B (π.supported_perm_of_support_map hπ h.hδ h.B S hS₁).to_struct_perm • L' =
-  struct_perm.derivative B (π.supported_perm hπ h H).to_struct_perm • L' :=
-begin
-  by_cases hflex : inflexible α L' B,
-  rw inflexible_iff at hflex,
-  obtain (⟨γ, δ, ε, hδ, hε, hδε, C, t, rfl, rfl⟩ | ⟨γ, ε, hε, C, a, rfl, rfl⟩) := hflex,
-  { have hc := λ c hc, ih _ (constrains.f_map hδ hε hδε C t c hc)
-      ⟨d, hd₁, relation.refl_trans_gen.head (constrains.f_map hδ hε hδε C t c hc) hd₂⟩,
-    have := (designated_support t).supports
-      ((allowable.derivative
-        (show path ((h.δ : Iic_index α) : type_index) (δ : Iic_index α), from C.cons (coe_lt hδ))
-        (π.supported_perm hπ h H))⁻¹ *
-      (allowable.derivative
-        (show path ((h.δ : Iic_index α) : type_index) (δ : Iic_index α), from C.cons (coe_lt hδ))
-        (π.supported_perm_of_support_map hπ h.hδ h.B S hS₁))) _,
-    { rw [mul_smul, inv_smul_eq_iff] at this,
-      rw [struct_perm.derivative_cons, struct_perm.derivative_bot_smul,
-        struct_perm.derivative_cons _ (C.cons _), struct_perm.derivative_bot_smul,
-        struct_perm.derivative_cons _ C, struct_perm.derivative_cons _ C],
-      rw allowable.derivative_to_struct_perm
-        (show path ((h.δ : Iic_index α) : type_index)
-          (⟨γ, coe_le_coe.mpr γ.prop⟩ : Iic_index α), from C),
-      rw allowable.derivative_to_struct_perm
-        (show path ((h.δ : Iic_index α) : type_index)
-          (⟨γ, coe_le_coe.mpr γ.prop⟩ : Iic_index α), from C),
-      have smul_f_map := to_struct_perm_smul_f_map (δ : Iio_index α) ε
-        (show (δ : type_index) < (⟨γ, coe_le_coe.mpr γ.prop⟩ : Iic_index α), from coe_lt hδ)
-        (coe_lt hε) (Iio.coe_injective.ne hδε),
-      exact (smul_f_map _ _).trans ((smul_f_map _ _).trans (congr_arg2 _ rfl this.symm)).symm, },
-    { intros d hd,
-      rw [mul_smul, inv_smul_eq_iff],
-      have := hc d hd,
-      rw [← allowable.to_struct_perm_smul, ← allowable.to_struct_perm_smul,
-        ← allowable.derivative_to_struct_perm, ← allowable.derivative_to_struct_perm],
-      refine prod.ext _ rfl,
-      change _ • _ = _ • _,
-      rw [struct_perm.derivative_derivative, struct_perm.derivative_derivative],
-      exact congr_arg prod.fst this, }, },
-  { have hc := ih _ (constrains.f_map_bot hε C a)
-      ⟨d, hd₁, relation.refl_trans_gen.head (constrains.f_map_bot hε C a) hd₂⟩,
-    rw [struct_perm.derivative_cons, struct_perm.derivative_bot_smul,
-      struct_perm.derivative_cons _ (C.cons _), struct_perm.derivative_bot_smul,
-      struct_perm.derivative_cons _ C, struct_perm.derivative_cons _ C],
-    rw allowable.derivative_to_struct_perm
-      (show path ((h.δ : Iic_index α) : type_index)
-        (⟨γ, coe_le_coe.mpr γ.prop⟩ : Iic_index α), from C),
-    rw allowable.derivative_to_struct_perm
-      (show path ((h.δ : Iic_index α) : type_index)
-        (⟨γ, coe_le_coe.mpr γ.prop⟩ : Iic_index α), from C),
-    have smul_f_map := to_struct_perm_smul_f_map (⊥ : Iio_index α) ε
-        (show ⊥ < (⟨γ, coe_le_coe.mpr γ.prop⟩ : Iic_index α), from bot_lt_coe _)
-        (coe_lt hε) (show (⊥ : Iio_index α) ≠ ε, from subtype.ne_of_val_ne bot_ne_coe),
-    refine (smul_f_map _ _).trans ((smul_f_map _ _).trans (congr_arg2 _ rfl _)).symm,
-    simp only,
-    have := supported_perm_smul_atom_eq π hπ h H S hS₁ hS₂ hS₃ d hd₁ _ a
-      (relation.refl_trans_gen.head (constrains.f_map_bot hε C a) hd₂),
-    -- Should be done, but instance diamonds make this goal very annoying to solve.
-    sorry, },
-  { rw [← struct_perm.of_bot_smul, ← struct_perm.of_bot_smul,
-      ← (supported_perm_exactly_approximates π hπ h H B).map_litter,
-      ← (supported_perm_of_support_map_exactly_approximates π hπ h.hδ h.B S hS₁ B).map_litter L' _,
-      supported_action_smul_litter_eq, supported_action_smul_litter_eq],
-    { by_cases L' ∈ (π ((h.B.cons _).comp B)).litter_perm.domain,
-      exact or.inl h,
-      exact or.inr ⟨hflex, h⟩, },
-    { by_cases L' ∈ (π ((h.B.cons _).comp B)).litter_perm.domain,
-      exact or.inl h,
-      exact or.inr ⟨hflex, h⟩, }, },
-end
-
-def support_map_supported (π : struct_approx β) (hπ : π.free)
-  {L : litter} {A : extended_index β} (h : inflexible_coe L A)
-  (H : hypothesis ⟨inr L.to_near_litter, A⟩) (S : support_map h.δ)
-  (hS₁ : (show struct_approx (h.δ : Iic α), from
-    supported_action S (λ (B : extended_index h.δ), π ((h.B.cons $ coe_lt h.hδ).comp B))).free) :=
-∀ (L : litter) (B : extended_index h.δ) (d : support_condition h.δ)
-  (hd₁ : d ∈ designated_support h.t)
-  (hd₂ : relation.refl_trans_gen (constrains α h.δ) (inr L.to_near_litter, B) d),
-  struct_perm.derivative B
-    (π.supported_perm_of_support_map hπ h.hδ h.B S hS₁).to_struct_perm • L =
-  struct_perm.derivative B
-    (π.supported_perm hπ h H).to_struct_perm • L →
-  struct_perm.derivative B
-    (π.supported_perm_of_support_map hπ h.hδ h.B S hS₁).to_struct_perm • L.to_near_litter =
-  struct_perm.derivative B
-    (π.supported_perm hπ h H).to_struct_perm • L.to_near_litter
-
-lemma supported_perm_smul_to_near_litter_eq (π : struct_approx β) (hπ : π.free)
-  {γ : Iic α} {δ : Iio α} (hδ : (δ : Λ) < γ) (B : path (β : type_index) γ) (S : support_map δ)
-  (hS : (show struct_approx (δ : Iic α), from supported_action S
-    (λ (C : extended_index δ), π ((B.cons $ coe_lt hδ).comp C))).free)
-  {L : litter} {C : extended_index δ} (hL : (inr L.to_near_litter, C) ∈ S)
-  (hS' : S.injective C)
-  (hL' : struct_perm.derivative C
-    (π.supported_perm_of_support_map hπ hδ B S hS).to_struct_perm • L =
-    (S.near_litter_image L.to_near_litter C hL).fst) :
-  struct_perm.derivative C
-    (π.supported_perm_of_support_map hπ hδ B S hS).to_struct_perm • L.to_near_litter =
-  S.near_litter_image L.to_near_litter C hL :=
-begin
-  refine set_like.coe_injective (set.ext (λ a, _)),
-  refine mem_smul_set.trans _,
-  simp only [litter.coe_to_near_litter, mem_litter_set, set_like.mem_coe,
-    struct_perm.to_near_litter_perm_smul],
-  split,
-  { rintro ⟨b, hb, rfl⟩,
-    by_cases hpreimage : without_preimage S (struct_perm.derivative C
-      (π.supported_perm_of_support_map hπ hδ B S hS).to_struct_perm • b) C,
-    { by_contradiction,
-      have : (struct_perm.derivative C
-          (π.supported_perm_of_support_map hπ hδ B S hS).to_struct_perm •
-          ((preimage_litter_equiv S C).symm ⟨_, hpreimage⟩ : atom)) =
-        (struct_perm.derivative C
-          (π.supported_perm_of_support_map hπ hδ B S hS).to_struct_perm • b),
-      { have := (supported_perm_of_support_map_exactly_approximates π hπ hδ B S hS C).map_atom _ _,
-        rw struct_perm.of_bot_smul at this,
-        rw ← this,
-        rw supported_action_smul_preimage_litter_equiv,
-        refl,
-        { exact hS', },
-        { rw supported_action_atom_perm_domain_eq,
-          exact or.inl (or.inl (or.inl (or.inr
-            ((preimage_litter_equiv S C).symm ⟨_, hpreimage⟩).prop))),
-          exact hS', }, },
-      rw smul_left_cancel_iff at this,
-      rw ← this at hb,
-      have := preimage_litter_subset_subset C ((preimage_litter_equiv S C).symm ⟨_, hpreimage⟩).prop,
-      rw [mem_litter_set, hb] at this,
-      have h₁ := preimage_litter_not_banned S C,
-      have h₂ := banned_litter.support_litter L hL,
-      rw this at h₂,
-      contradiction, },
-    rw without_preimage_iff at hpreimage,
-    simp only [mem_litter_set, ne.def, not_and, not_forall, not_not, bex_imp_distrib] at hpreimage,
-    by_cases hb' : b ∈ supported_action_atom_map_core_domain S C,
-    { have := (supported_perm_of_support_map_exactly_approximates π hπ hδ B S hS C).map_atom b _,
-      rw struct_perm.of_bot_smul at this,
-      rw ← this,
-      clear this,
-      obtain ((hb' | hb') | hb') := hb',
-      { rw supported_action_smul_atom_eq _ _ _ _ hb' hS',
-        -- Need an assumption on `S`.
-        sorry },
-      { cases eq_of_mem_litter_set_of_mem_litter_set hb (preimage_litter_subset_subset C hb'),
-        cases preimage_litter_not_banned S C (banned_litter.support_litter _ hL), },
-      { simp only [mem_Union] at hb',
-        obtain ⟨L', hL', hbL'⟩ := hb',
-        cases eq_of_mem_litter_set_of_mem_litter_set hb
-          (mapped_outside_subset_subset L' C hL' hbL'),
-        rw supported_action_smul_of_mem_mapped_outside_subset _ _ _ hbL' hS',
-        exact (mapped_outside_equiv S L C hL' ⟨b, hbL'⟩).prop.mem_map, },
-      { rw supported_action_atom_perm_domain_eq,
-        exact or.inl (or.inl hb'),
-        exact hS', }, },
-    have himage : ∀ (c : atom) (hc : (inl c, C) ∈ S.carrier),
-      struct_perm.derivative C (π.supported_perm_of_support_map hπ hδ B S hS).to_struct_perm • b ≠
-      S.atom_image c C hc,
-    { intros c hc hbc,
-      have := (supported_perm_of_support_map_exactly_approximates π hπ hδ B S hS C).map_atom c _,
-      rw [struct_perm.of_bot_smul, supported_action_smul_atom_eq, ← hbc,
-        smul_left_cancel_iff] at this,
-      cases this,
-      exact hb' (or.inl (or.inl hc)),
-      { exact hS', },
-      { rw supported_action_atom_perm_domain_eq _ hS',
-        exact or.inl (or.inl (or.inl (or.inl hc))), }, },
-    by_cases hb'' : b ∈
-      (supported_action S (λ C, π ((B.cons $ coe_lt hδ).comp C)) C).atom_perm.domain,
-    { rw supported_action_atom_perm_domain_eq at hb'',
-      obtain ((hb'' | hb'') | hb'') := hb'',
-      { cases hb' hb'', },
-      { rw mem_image at hb'',
-        obtain ⟨c, hc, hbc⟩ := hb'',
-        sorry,
-        -- obtain ⟨c, (hc | hc) | hc, hbc⟩ := hb'',
-        -- {  },
-         },
-      { cases eq_of_mem_litter_set_of_mem_litter_set hb (local_perm.sandbox_subset_subset _ _ hb''),
-        cases sandbox_litter_not_banned S C (banned_litter.support_litter _ hL), },
-      { exact hS', }, },
-    have hlitter := (supported_perm_of_support_map_exactly_approximates
-      π hπ hδ B S hS C).mem_litter_set b hb'',
-    rw [hb, struct_perm.of_bot_smul, struct_perm.of_bot_smul, hL'] at hlitter,
-    have := mt (hpreimage L hL hlitter),
-    clear hpreimage,
-    simp only [not_exists, not_forall, not_not] at this,
-    obtain ⟨L', hL', hbL'⟩ := this himage,
-    by_cases hLL' : L = L',
-    { cases hLL',
-      exact hbL', },
-    have houtside := mapped_outside.mk hbL'
-      (λ h, hLL' (hS'.near_litter_injective hL hL'
-        (near_litter.inter_nonempty_of_fst_eq_fst
-          (eq_of_mem_litter_set_of_mem_litter_set hlitter h)))) himage,
-    have : (struct_perm.derivative C
-        (π.supported_perm_of_support_map hπ hδ B S hS).to_struct_perm •
-        ((mapped_outside_equiv S L' C hL').symm ⟨_, houtside⟩ : atom)) =
-      struct_perm.derivative C
-        (π.supported_perm_of_support_map hπ hδ B S hS).to_struct_perm • b,
-    { have := (supported_perm_of_support_map_exactly_approximates π hπ hδ B S hS C).map_atom _ _,
-      rw struct_perm.of_bot_smul at this,
-      rw ← this,
-      rw supported_action_smul_mapped_outside_equiv,
-      refl,
-      { exact hS', },
-      { rw supported_action_atom_perm_domain_eq _ hS',
-        refine or.inl (or.inl (or.inr _)),
-        simp only [mem_Union],
-        exact ⟨L', hL', ((mapped_outside_equiv S L' C hL').symm ⟨_, houtside⟩).prop⟩, }, },
-    rw smul_left_cancel_iff at this,
-    rw ← this at hb,
-    have := mapped_outside_subset_subset L' C hL'
-      ((mapped_outside_equiv S L' C hL').symm ⟨_, houtside⟩).prop,
-    rw [mem_litter_set, hb] at this,
-    have h₁ := preimage_litter_not_banned S C,
-    have h₂ := banned_litter.support_litter L hL,
-    rw this at h₂,
-    contradiction, },
-  { intro ha,
-    by_cases himage : ∃ (b : atom) (hb : (inl b, C) ∈ S.carrier),
-      struct_perm.derivative C (π.supported_perm_of_support_map hπ hδ B S hS).to_struct_perm • a =
-      S.atom_image b C hb,
-    { obtain ⟨b, hb, hab⟩ := himage,
-      have : a = b,
-      { have := (supported_perm_of_support_map_exactly_approximates π hπ hδ B S hS C).map_atom b _,
-        have := hab.trans ((supported_action_smul_atom_eq _ _ _ _ _ _).symm.trans this),
-        simp only [struct_perm.of_bot_smul, smul_left_cancel_iff] at this,
-        exact this,
-        exact hS',
-        rw supported_action_atom_perm_domain_eq _ hS',
-        exact or.inl (or.inl (or.inl (or.inl hb))), },
-      cases this,
-      refine ⟨(struct_perm.derivative C
-        (π.supported_perm_of_support_map hπ hδ B S hS).to_struct_perm)⁻¹ • a, _, _⟩,
-      { -- Need an assumption on S.
-        sorry, },
-      { rw smul_inv_smul, }, },
-    simp only [not_exists] at himage,
-    by_cases himage' : ∃ (b : atom) (hb : (inl b, C) ∈ S.carrier),
-      a = S.atom_image b C hb,
-    { obtain ⟨b, hb, hab⟩ := himage',
-      refine ⟨b, _, _⟩,
-      { -- Need an assumption on S.
-        sorry, },
-      { have := (supported_perm_of_support_map_exactly_approximates π hπ hδ B S hS C).map_atom b _,
-        have := hab.trans ((supported_action_smul_atom_eq _ _ _ _ _ _).symm.trans this),
-        rw struct_perm.of_bot_smul at this,
-        exact this.symm,
-        exact hS',
-        rw supported_action_atom_perm_domain_eq _ hS',
-        exact or.inl (or.inl (or.inl (or.inl hb))), }, },
-    by_cases houtside : mapped_outside S L C hL a,
-    { refine ⟨(mapped_outside_equiv S L C hL).symm ⟨_, houtside⟩,
-        mapped_outside_subset_subset L C hL
-          ((mapped_outside_equiv S L C hL).symm ⟨_, houtside⟩).prop, _⟩,
-      have := (supported_perm_of_support_map_exactly_approximates π hπ hδ B S hS C).map_atom _ _,
-      rw struct_perm.of_bot_smul at this,
-      rw [← this, supported_action_smul_mapped_outside_equiv],
-      refl,
-      exact hS',
-      rw supported_action_atom_perm_domain_eq _ hS',
-      refine or.inl (or.inl (or.inr _)),
-      simp only [mem_Union],
-      exact ⟨_, _, ((mapped_outside_equiv S L C hL).symm ⟨_, houtside⟩).prop⟩, },
-    { simp only [mapped_outside_iff, set_like.mem_coe, mem_litter_set, ne.def, not_and,
-        not_forall, not_not] at houtside,
-      have haL := not_not.mp (mt (houtside ha) (by simpa only using himage')),
-      refine ⟨_, _, smul_inv_smul _ _⟩,
-      -- Use `ha` and an assumption on S.
-      sorry, }, },
-end
-
-lemma supported_perm_smul_near_litter_eq (π : struct_approx β) (hπ : π.free)
-  {L : litter} {A : extended_index β} (h : inflexible_coe L A)
-  (H : hypothesis ⟨inr L.to_near_litter, A⟩) (S : support_map h.δ)
-  (hS₁ : (show struct_approx (h.δ : Iic α), from
-    supported_action S (λ (B : extended_index h.δ), π ((h.B.cons $ coe_lt h.hδ).comp B))).free)
-  (hS₂ : inflexible_support_map H h ≤ S) (hS₃ : ∀ B, S.injective B)
-  (hS₄ : support_map_supported π hπ h H S hS₁)
-  (d : support_condition h.δ) (hd₁ : d ∈ designated_support h.t)
-  (B : extended_index h.δ) (N : near_litter)
-  (ih : ∀ (y : support_condition h.δ), y ≺[α] (inr N, B) →
-    (∃ d ∈ designated_support h.t, relation.refl_trans_gen (constrains α h.δ) y d) →
-    π.supported_perm_of_support_map hπ h.hδ h.B S hS₁ • y =
-      π.supported_perm hπ h H • y)
-  (hd₂ : relation.refl_trans_gen (constrains α h.δ) (inr N, B) d) :
-  struct_perm.derivative B (π.supported_perm_of_support_map hπ h.hδ h.B S hS₁).to_struct_perm • N =
-  struct_perm.derivative B (π.supported_perm hπ h H).to_struct_perm • N :=
-begin
-  by_cases hN : N.is_litter,
-  { obtain ⟨L', rfl⟩ := hN.exists_litter_eq,
-    exact hS₄ L' B d hd₁ hd₂
-      (supported_perm_smul_litter_eq π hπ h H S hS₁ hS₂ hS₃ d hd₁ B L' ih hd₂), },
-  have hL : (_, _) = (_, _) := ih _ (constrains.near_litter N (near_litter.not_is_litter hN) B)
-    ⟨d, hd₁, relation.refl_trans_gen.head
-      (constrains.near_litter N (near_litter.not_is_litter hN) B) hd₂⟩,
-  have ha := λ a ha, ih _ (constrains.symm_diff N a ha B)
-    ⟨d, hd₁, relation.refl_trans_gen.head (constrains.symm_diff N a ha B) hd₂⟩,
-  change ∀ a h, (_, _) = (_, _) at ha,
-  simp only [smul_inl, smul_inr, prod.mk.inj_iff, eq_self_iff_true, and_true] at hL ha,
-  refine set_like.coe_injective _,
-  refine (near_litter_perm.smul_near_litter_eq_smul_symm_diff_smul _ _).trans
-    ((near_litter_perm.smul_near_litter_eq_smul_symm_diff_smul _ _).trans _).symm,
-  simp only [struct_perm.to_near_litter_perm_smul, litter.coe_to_near_litter],
-  congr' 1,
-  { exact congr_arg (λ (N : near_litter), (N.2 : set atom)) hL.symm, },
-  ext a : 1,
-  simp only [struct_perm.to_near_litter_perm_smul, mem_smul_set_iff_inv_smul_mem],
-  split,
-  { intro ha',
-    have := (ha _ ha').trans (smul_inv_smul _ _),
-    rw smul_eq_iff_eq_inv_smul at this,
-    refine mem_of_eq_of_mem _ ha',
-    simp only [← map_inv] at this ⊢,
-    exact this.symm, },
-  { intro ha',
-    have := (ha _ ha').symm.trans (smul_inv_smul _ _),
-    rw smul_eq_iff_eq_inv_smul at this,
-    refine mem_of_eq_of_mem _ ha',
-    simp only [← map_inv] at this ⊢,
-    exact this.symm, },
-end
-
-lemma supported_perm_smul_condition_eq (π : struct_approx β) (hπ : π.free)
-  {L : litter} {A : extended_index β} (h : inflexible_coe L A)
-  (H : hypothesis ⟨inr L.to_near_litter, A⟩) (S : support_map h.δ)
-  (hS₁ : (show struct_approx (h.δ : Iic α), from
-    supported_action S (λ (B : extended_index h.δ), π ((h.B.cons $ coe_lt h.hδ).comp B))).free)
-  (hS₂ : inflexible_support_map H h ≤ S)
-  (hS₃ : ∀ B, S.injective B)
-  (hS₄ : support_map_supported π hπ h H S hS₁)
-  {c : support_condition h.δ} :
-  (∃ d ∈ designated_support h.t, relation.refl_trans_gen (constrains α h.δ) c d) →
-  supported_perm_of_support_map π hπ h.hδ h.B S hS₁ • c = supported_perm π hπ h H • c :=
-begin
-  refine (constrains_wf α h.δ).induction c _,
-  rintros c ih ⟨d, hd₁, hd₂⟩,
-  obtain ⟨a | N, B⟩ := c,
-  { refine prod.ext _ rfl,
-    change inl _ = inl _,
-    exact congr_arg inl (supported_perm_smul_atom_eq π hπ h H S hS₁ hS₂ hS₃ d hd₁ B a hd₂), },
-  { refine prod.ext _ rfl,
-    change inr _ = inr _,
-    exact congr_arg inr
-      (supported_perm_smul_near_litter_eq π hπ h H S hS₁ hS₂ hS₃ hS₄ d hd₁ B N ih hd₂), },
-end
-
-/-- As long as a support map extends the `inflexible_support_map`, the supported action generated
-by this map agrees with the supported action generated by the `inflexible_support_map` on `t`. -/
-lemma supported_perm_smul_eq (π : struct_approx β) (hπ : π.free)
-  {L : litter} {A : extended_index β} (h : inflexible_coe L A)
-  (H : hypothesis ⟨inr L.to_near_litter, A⟩) (S : support_map h.δ)
-  (hS₁ : (show struct_approx (h.δ : Iic α), from
-    supported_action S (λ (B : extended_index h.δ), π ((h.B.cons $ coe_lt h.hδ).comp B))).free)
-  (hS₂ : inflexible_support_map H h ≤ S)
-  (hS₃ : ∀ B, S.injective B)
-  (hS₄ : support_map_supported π hπ h H S hS₁) :
-  supported_perm π hπ h H • h.t = supported_perm_of_support_map π hπ h.hδ h.B S hS₁ • h.t :=
-begin
-  rw [smul_eq_iff_eq_inv_smul, smul_smul],
-  symmetry,
-  refine (designated_support h.t).supports _ _,
-  intros c hc,
-  rw [mul_smul, inv_smul_eq_iff],
-  exact supported_perm_smul_condition_eq π hπ h H S hS₁ hS₂ hS₃ hS₄
-    ⟨c, hc, relation.refl_trans_gen.refl⟩,
-end-/
 
 noncomputable def litter_completion (π : struct_approx β) (hπ : π.free)
   (L : litter) (A : extended_index β) (H : hypothesis ⟨inr L.to_near_litter, A⟩) : litter :=
