src/phase2/refine.lean
@@ -1,0 +1,59 @@
+import phase2.fill_atom_range
+import phase2.fill_atom_orbits
+
+universe u
+
+namespace con_nf
+variables [params.{u}]
+
+/-!
+# Refinements of weak approximations
+-/
+
+namespace weak_near_litter_approx
+
+variables (w : weak_near_litter_approx)
+
+noncomputable def refine : weak_near_litter_approx :=
+w.fill_atom_range.fill_atom_orbits fill_atom_range_symm_diff_subset_ran
+
+variable {w}
+
+@[simp] lemma refine_atom_map {a : atom} (ha : (w.atom_map a).dom) :
+  w.refine.atom_map a = w.atom_map a :=
+begin
+  unfold refine,
+  refine part.ext' _ _,
+  { simp only [ha, fill_atom_orbits_atom_map, orbit_atom_map_dom_iff, fill_atom_range_atom_map,
+      iff_true],
+    exact or.inl (or.inl ha), },
+  intros h₁ h₂,
+  refine (w.fill_atom_range.orbit_atom_map_eq_of_mem_dom _ (or.inl ha)).trans _,
+  exact w.supported_action_eq_of_dom ha,
+end
+
+@[simp] lemma refine_litter_map : w.refine.litter_map = w.litter_map := rfl
+
+lemma refine_precise : precise w.refine :=
+fill_atom_orbits_precise fill_atom_range_symm_diff_subset_ran
+
+end weak_near_litter_approx
+
+namespace weak_struct_approx
+
+variables {β : type_index} (w : weak_struct_approx β)
+
+noncomputable def refine : weak_struct_approx β := λ A, (w A).refine
+
+@[simp] lemma refine_atom_map {A : extended_index β} {a : atom} (ha : ((w A).atom_map a).dom) :
+  (w A).refine.atom_map a = (w A).atom_map a := weak_near_litter_approx.refine_atom_map ha
+
+@[simp] lemma refine_litter_map {A : extended_index β} :
+  (w A).refine.litter_map = (w A).litter_map := rfl
+
+lemma refine_precise {A : extended_index β} : precise w.refine :=
+λ A, weak_near_litter_approx.refine_precise
+
+end weak_struct_approx
+
+end con_nf
